Setlec/SetR.lean
@@ -93,6 +93,7 @@ import Setlec.SetR.Interp2.Step2.Fuel
 import Setlec.SetR.Interp2.Step2.InferQ
 import Setlec.SetR.Interp2.Claims2A
 import Setlec.SetR.Interp2.EnvS2Refute
+import Setlec.SetR.Interp2.Claims2B
 import Setlec.SetR.Annot.Canon
 import Setlec.SetR.Annot.SimSubst
 import Setlec.SetR.Annot.PremiseLadder
